working on custom distinct tactic

Geometry/Theory/Distinct.lean
@@ -10,25 +10,77 @@ namespace Geometry.Theory.Distinct
 
 open Set
 
+open Lean Meta Expr Elab.Tactic Qq
+
+
+-- idea: when this is called, assume the main goal is of the form
+-- A ≠ B ∧ ...
+-- search for any `distinct` blocks floating around and attempt to refine the goal
+-- as much as possible, so ideally a proof like:
+--
+-- h : distinct A B C D E := by magic
+-- ⊢ A ≠ B ∧ B ≠ E ∧ X ≠ A
+--
+-- runDistinguish should satisfy the first two and leave the last one.
+--
+
+structure Distinct {α : Type*} (points : List α) : Prop where
+  pairwise : List.Pairwise (· ≠ ·) points
+
 -- Custom syntax category for the distinct binder
 declare_syntax_cat distinct_binder
 syntax ident+ " : " term : distinct_binder
 
-syntax "distinct " ident+ : term
+syntax "distinct" ident+ : term
 macro_rules
-  | `(distinct $[$xs]*) => do
-    `(List.Pairwise (· ≠ ·) [$[$xs],*])
+  | `(distinct $xs*) => `(Distinct [$xs,*])
 
-open Lean Elab Tactic Meta in
-elab "distinguish" h:ident x:ident y:ident : tactic => do
-  evalTactic (← `(tactic| (
-    have : $x:ident ≠ $y:ident := by
-      simp only [List.pairwise_cons, List.mem_cons] at $h:ident
-      -- FIXME: I don't love the simp_all here, it's better than a bare simp_all but
-      -- I feel like there is a way to more systematically prove this
-      simp_all
-    try assumption
-  )))
+/-- Extracts a list of expressions like `X ≠ Y ∧ ...` into [ X≠Y, ...] -/
+partial def extractIneqs (e : Expr) : MetaM (List Expr) := do
+  have qe : Q(Prop) := e
+  match qe with
+  | ~q(@And $lhs $rhs) => do
+    let lhsIneqs ← extractIneqs lhs
+    let rhsIneqs ← extractIneqs rhs
+    return lhsIneqs ++ rhsIneqs
+  | ~q(@Ne _ $a $b) =>
+    return [e]
+  | _ => return []
+
+/-- Finds all `Distinct` hypotheses in the local context -/
+def findDistinctHypos : TacticM (List Expr) := do
+  withMainContext do
+    let lctx ← getLCtx
+    let mut distinctHypos : List Expr := []
+    for decl in lctx do
+      if decl.isImplementationDetail then continue
+      let declType ← instantiateMVars decl.type
+      if declType.isAppOfArity ``Distinct 2 then
+        distinctHypos := decl.toExpr :: distinctHypos
+    return distinctHypos
+
+
+def runDistinguish : TacticM Unit := do
+  withMainContext do
+    let tgt ← getMainTarget
+    let ineqs ← extractIneqs tgt
+    logInfo m!"{ineqs}"
+    --
+    let distinctHypos ← findDistinctHypos
+    logInfo m!"found hypos {distinctHypos}"
+ 
+    --
+    throwError "test"
+
+example : Distinct [A, B, C, D, E] -> A ≠ B ∧ B ≠ C ∧ X ≠ A ∧ (∀ P : Nat, P > 1) ∧ C ≠ D := by
+  intro h
+  run_tac runDistinguish -- should be A≠B, B≠C, X≠A, C≠D
+  sorry
+
+example : distinct A B C D E -> A ≠ B ∧ B ≠ C ∧ X ≠ A ∧ (∀ P : Nat, P > 1) ∧ C ≠ D := by
+  intro h
+  run_tac runDistinguish -- should be A≠B, B≠C, X≠A, C≠D
+  sorry
 
 -- TODO: Make the `h` optional by searching the proofstate
 -- TODO: Maybe make the X and Y optional as well
